Nemonuri/Functions/LiftableEmbedding/Set.lean
@@ -1,0 +1,97 @@
+module
+
+public import Nemonuri.Functions.LiftableEmbedding.Basic
+
+@[expose] public section
+
+set_option autoImplicit false
+
+namespace Nemonuri.Functions.LiftableEmbedding
+
+
+variable {L R: Type*}
+
+def embedSet (lem: LiftableEmbedding L R) (s: Set L) : Set R := { rv: R | lem.embedPred (· ∈ s) rv }
+
+theorem embedSet_mem_iff (lem: LiftableEmbedding L R) {s: Set L} {rv: R}
+  : (rv ∈ lem.embedSet s) ↔ (∃(req: lem.IsLiftable rv), req.lift ∈ s) := by
+  dsimp [embedSet, embedPred]
+  simp only [dite_else_false]
+
+theorem embedSet_injective {lem: LiftableEmbedding L R} : Function.Injective (lem.embedSet) := by
+  intro s1 s2 lm1
+  rewrite [Set.ext_iff] at ⊢ lm1
+  intro lv
+  specialize lm1 (lem lv)
+  simp [embedSet_mem_iff, IsLiftable.of_apply] at lm1
+  exact IsLiftable.pred_lift_iff_iff_self_iff.mp lm1
+
+
+def liftSet (lem: LiftableEmbedding L R) (s: Set R) : Set L := { lv: L | lem.liftPred (· ∈ s) lv }
+
+theorem liftSet_embedSet_leftInverse {lem: LiftableEmbedding L R} : Function.LeftInverse lem.liftSet lem.embedSet := by
+  intro sl
+  dsimp [liftSet, embedSet]
+  rw [lem.liftPred_embedPred_leftInverse.eq]
+  exact Set.setOf_mem_eq
+
+theorem liftSet_surjective {lem: LiftableEmbedding L R} : Function.Surjective lem.liftSet := lem.liftSet_embedSet_leftInverse.surjective
+
+--theorem liftSet_injective {lem: LiftableEmbedding L R}
+
+
+theorem liftSet_mem_iff (lem: LiftableEmbedding L R) {s: Set R} {lv: L}
+  : (lv ∈ lem.liftSet s) ↔ (lem lv ∈ s) := by
+  dsimp [liftSet, liftPred]
+  exact Iff.rfl
+
+
+def ofSet (lem: LiftableEmbedding L R) : LiftableEmbedding (Set L) (Set R) where
+  embed := lem.embedSet
+  lift s _ := lem.liftSet s
+  valid := by
+    refine .mk ?_
+    dsimp [RestrictedLeftInverse]
+    exact lem.liftSet_embedSet_leftInverse
+
+theorem set_elem_isLiftable_of_ofSet_isLiftable {lem: LiftableEmbedding L R} {rs: Set R} (req: lem.ofSet.IsLiftable rs) (rv: rs) : lem.IsLiftable rv.val := by
+  revert rv
+  simp only [Subtype.forall]
+  intro rv lm1
+  simp [isLiftable_iff_left_exists] at req
+  rcases req with ⟨ls, lm2⟩
+  dsimp [coe_def, ofSet] at lm2
+  subst lm2
+  simp [embedSet_mem_iff] at lm1
+  rcases lm1 with ⟨lm1, _⟩
+  exact lm1
+
+
+theorem ofSet_isLiftable_iff {lem: LiftableEmbedding L R} {rs: Set R}
+  : (lem.ofSet.IsLiftable rs) ↔ (∀(rv: rs), lem.IsLiftable rv.val) := by
+  constructor
+  · exact lem.set_elem_isLiftable_of_ofSet_isLiftable
+  · simp only [Subtype.forall]
+    intro lm1
+    simp [isLiftable_iff_left_exists]
+    exists (lem.liftSet rs)
+    dsimp [coe_def, ofSet]
+    simp [Set.ext_iff]
+    intro rv
+    simp [embedSet_mem_iff, liftSet_mem_iff]
+    conv => rhs; arg 1; ext; arg 2; simp [IsLiftable.lift_apply_eq_self]
+    simp
+    exact lm1 rv
+
+
+
+
+
+/-
+instance (lem: LiftableEmbedding L R) : DecidablePred (lem.ofSet.IsLiftable ·) := fun _ => .isTrue (by
+  simp [isLiftable_iff_left_exists])
+-/
+
+end Nemonuri.Functions.LiftableEmbedding
+
+end
